src/cbor/pulse/CBOR.Pulse.API.Base.fst
@@ -8,7 +8,6 @@ module SZ = FStar.SizeT
 module U64 = FStar.UInt64
 module U8 = FStar.UInt8
 module R = Pulse.Lib.Reference
-module A = Pulse.Lib.Array
 module PM = Pulse.Lib.SeqMatch
 
 (** Destructors *)
@@ -539,22 +538,21 @@ inline_for_extraction
 let mk_array_t
   (#t: Type)
   (vmatch: perm -> t -> cbor -> slprop)
-= (a: A.array t) ->
-  (len: U64.t) ->
+= (a: S.slice t) ->
   (#pa: perm) ->
   (#va: Ghost.erased (Seq.seq t)) ->
   (#pv: perm) ->
   (#vv: Ghost.erased (list cbor)) ->
   stt t
-    (A.pts_to a #pa va **
+    (pts_to a #pa va **
       PM.seq_list_match va vv (vmatch pv) **
-      pure (U64.v len == Seq.length va)
+      pure (FStar.UInt.fits (SZ.v (S.len a)) U64.n)
     )
     (fun res -> exists* p' v' .
       vmatch p' res (pack (CArray v')) **
       Trade.trade
         (vmatch p' res (pack (CArray v')))
-        (A.pts_to a #pa va **
+        (pts_to a #pa va **
           PM.seq_list_match va vv (vmatch pv)
         ) **
         pure (v' == Ghost.reveal vv)
@@ -565,15 +563,14 @@ let mk_map_t
   (#t1 #t2: Type)
   (vmatch1: perm -> t1 -> cbor -> slprop)
   (vmatch2: perm -> t2 -> (cbor & cbor) -> slprop)
-= (a: A.array t2) ->
-  (len: U64.t) ->
+= (a: S.slice t2) ->
   (#va: Ghost.erased (Seq.seq t2)) ->
   (#pv: perm) ->
   (#vv: Ghost.erased (list (cbor & cbor))) ->
   stt t1
-    (A.pts_to a va **
+    (pts_to a va **
       PM.seq_list_match va vv (vmatch2 pv) **
-      pure (U64.v len == Seq.length va /\
+      pure (FStar.UInt.fits (SZ.v (S.len a)) U64.n /\
         List.Tot.no_repeats_p (List.Tot.map fst vv)
       )
     )
@@ -581,7 +578,7 @@ let mk_map_t
       vmatch1 p' res (pack (CMap v')) **
       Trade.trade
         (vmatch1 p' res (pack (CMap v')))
-        (A.pts_to a va' ** // this function potentially sorts the input array, so we lose the link to the initial array contents
+        (pts_to a va' ** // this function potentially sorts the input array, so we lose the link to the initial array contents
           PM.seq_list_match va vv (vmatch2 pv) // but we keep the permissions on each element
         ) **
         pure (
