src/cbor/spec/raw/CBOR.Spec.Raw.fsti
@@ -88,6 +88,12 @@ let mk_det_raw_cbor_map_entry
 : Tot (R.raw_data_item & R.raw_data_item)
 = (mk_det_raw_cbor (fst x), mk_det_raw_cbor (snd x))
 
+val no_repeats_map_fst_mk_det_raw_cbor_map_entry
+  (l: list (cbor & cbor))
+: Lemma
+  (requires (List.Tot.no_repeats_p (List.Tot.map fst l)))
+  (ensures (List.Tot.no_repeats_p (List.Tot.map fst (List.Tot.map mk_det_raw_cbor_map_entry l))))
+
 val mk_det_raw_cbor_map
   (l: list (cbor & cbor))
   (len: FStar.UInt64.t)
